Split wip; a temporal commit for experiments

src/Split.v
@@ -1,8 +1,11 @@
 Require Import List String.
-Require Import Lib.CommonTactics Lib.FMap.
+Require Import Lib.CommonTactics Lib.Struct Lib.FMap.
 Require Import Syntax Semantics SemFacts.
 
 Set Implicit Arguments.
+
+Definition emptyLabel: LabelT :=
+  {| annot := None; defs := M.empty _; calls := M.empty _ |}.
 
 Fixpoint composeLabels (ls1 ls2: LabelSeqT) :=
   match ls1, ls2 with
@@ -11,49 +14,200 @@ Fixpoint composeLabels (ls1 ls2: LabelSeqT) :=
     | _, _ => nil
   end.
 
-Lemma multistep_split:
-  forall ma mb s ls ir,
-    Multistep (ConcatMod ma mb) ir s ls ->
-    ir = initRegs (getRegInits ma ++ getRegInits mb) ->
-    exists sa lsa sb lsb,
-      Multistep ma (initRegs (getRegInits ma)) sa lsa /\
-      Multistep mb (initRegs (getRegInits mb)) sb lsb /\
-      s = M.union sa sb /\ ls = composeLabels lsa lsb.
+Lemma substep_regs_new:
+  forall m o u ul cs,
+    Substep m o u ul cs -> M.KeysSubset u (namesOf (getRegInits m)).
 Proof.
-  induction 1.
-  - do 2 (eexists; exists nil); repeat split; try constructor.
-    subst. admit.
-
-  - intros; subst.
-    specialize (IHMultistep eq_refl).
-    destruct IHMultistep as [sa [lsa [sb [lsb [? [? [? ?]]]]]]]; subst.
-    admit.
+  induction 1; auto.
+  - apply M.KeysSubset_empty.
+  - apply M.KeysSubset_empty.
+  - admit. (* easy but tedious *)
+  - admit. (* easy but tedious *)
 Qed.
 
-Lemma behavior_split:
-  forall ma mb s ls,
-    Behavior (ConcatMod ma mb) s ls ->
-    exists sa lsa sb lsb,
-      Behavior ma sa lsa /\ Behavior mb sb lsb /\
-      s = M.union sa sb /\
-      ls = composeLabels lsa lsb. 
-Proof.
-  induction 1.
-  apply multistep_split in HMultistepBeh.
-  destruct HMultistepBeh as [sa [lsa [sb [lsb [? [? [? ?]]]]]]]; subst.
-  exists sa, lsa, sb, lsb.
-  repeat split; auto.
-  reflexivity.
-Qed.
-
-Lemma behavior_modular:
-  forall ma mb sa sb lsa lsb,
-    Behavior ma sa lsa ->
-    Behavior mb sb lsb ->
-    Behavior (ConcatMod ma mb) (M.union sa sb) (composeLabels lsa lsb).
+Lemma substepsInd_regs_new:
+  forall m o u l,
+    SubstepsInd m o u l -> M.KeysSubset u (namesOf (getRegInits m)).
 Proof.
   admit.
 Qed.
+
+Lemma step_regs_new:
+  forall m o u l,
+    Step m o u l -> M.KeysSubset u (namesOf (getRegInits m)).
+Proof.
+  intros; apply step_consistent in H.
+  induction H.
+  eapply substepsInd_regs_new; eauto.
+Qed.
+
+Lemma multistep_regs:
+  forall m s ls ir,
+    Multistep m ir s ls ->
+    ir = initRegs (getRegInits m) ->
+    M.KeysSubset s (namesOf (getRegInits m)).
+Proof.
+  induction 1; simpl; intros; subst.
+  - admit. (* easy *)
+  - apply M.KeysSubset_union; auto.
+    eapply step_regs_new; eauto.
+Qed.
+
+Section TwoModules.
+  Variables (ma mb: Modules).
+  Hypothesis (Hinit: DisjList (namesOf (getRegInits ma)) (namesOf (getRegInits mb))).
+
+  Definition mergeUnitLabel (ul1 ul2: UnitLabel): UnitLabel :=
+    match ul1, ul2 with
+      | _, Rle _ => ul2
+      | _, _ => ul1
+    end.
+
+  Lemma substep_split:
+    forall o u ul cs,
+      Substep (ConcatMod ma mb) o u ul cs ->
+      exists oa ob ua ub ula ulb csa csb,
+        Substep ma oa ua ula csa /\ Substep mb ob ub ulb csb /\
+        o = M.union oa ob /\ u = M.union ua ub /\
+        ul = mergeUnitLabel ula ulb /\ cs = M.union csa csb.
+  Proof.
+    induction 1; simpl; intros.
+
+    - 
+  Qed.
+
+  Lemma substepsInd_split:
+    forall o u l,
+      SubstepsInd (ConcatMod ma mb) o u l ->
+      exists oa ob ua ub la lb,
+        SubstepsInd ma oa ua la /\ SubstepsInd mb ob ub lb /\
+        o = M.union oa ob /\ u = M.union ua ub /\ l = mergeLabel la lb.
+  Proof.
+    induction 1; simpl; intros.
+    - exists o, (M.empty _), (M.empty _), (M.empty _), emptyLabel, emptyLabel.
+      repeat split; auto; constructor.
+
+    - subst.
+      destruct IHSubstepsInd as [poa [pob [pua [pub [pla [plb ?]]]]]]; dest; subst.
+      apply substep_split in H0.
+      destruct H0 as [soa [sob [sua [sub [sula [sulb [scsa [scsb ?]]]]]]]]; dest; subst.
+
+      exists poa, pob, (M.union pua sua), (M.union pub sub).
+      exists (mergeLabel (getLabel sula scsa) pla), (mergeLabel (getLabel sulb scsb) plb).
+
+      repeat split.
+
+      + eapply SubstepsCons; eauto.
+        * assert (poa = soa) by admit; subst. (* map stuff *)
+          auto.
+        * inv H1; dest.
+          repeat split; auto.
+          { mdisj. admit. }
+          { admit. }
+
+      + eapply SubstepsCons; eauto.
+        * assert (pob = sob) by admit; subst. (* map stuff *)
+          auto.
+        * inv H1; dest.
+          repeat split; auto.
+          { mdisj. admit. }
+          { admit. }
+
+      + inv H1; auto.
+      + admit.
+  Qed.
+
+  Lemma stepInd_split:
+    forall o u l,
+      StepInd (ConcatMod ma mb) o u l ->
+      exists oa ob ua ub la lb,
+        StepInd ma oa ua la /\ StepInd mb ob ub lb /\
+        o = M.union oa ob /\ u = M.union ua ub /\ l = hide (mergeLabel la lb).
+  Proof.
+    induction 1; simpl; intros.
+    pose proof (substepsInd_split HSubSteps)
+      as [oa [ob [ua [ub [la [lb ?]]]]]]; dest; subst.
+    exists oa, ob, ua, ub, (hide la), (hide lb).
+    intuition auto.
+
+    - constructor; auto.
+      admit. (* maybe the most difficult part *)
+    - constructor; auto.
+      admit. (* maybe the most difficult part *)
+    - admit. (* easy, using hide_idempotent *)
+  Qed.
+
+  Lemma step_split:
+    forall o u l,
+      Step (ConcatMod ma mb) o u l ->
+      exists oa ob ua ub la lb,
+        Step ma oa ua la /\ Step mb ob ub lb /\
+        o = M.union oa ob /\ u = M.union ua ub /\ l = hide (mergeLabel la lb).
+  Proof.
+    intros; apply step_consistent in H.
+    pose proof (stepInd_split H) as [oa [ob [ua [ub [la [lb ?]]]]]]; dest; subst.
+    exists oa, ob, ua, ub, la, lb.
+    repeat split; apply step_consistent; auto.
+  Qed.
+
+  Lemma multistep_split:
+    forall s ls ir,
+      Multistep (ConcatMod ma mb) ir s ls ->
+      ir = initRegs (getRegInits ma ++ getRegInits mb) ->
+      exists sa lsa sb lsb,
+        Multistep ma (initRegs (getRegInits ma)) sa lsa /\
+        Multistep mb (initRegs (getRegInits mb)) sb lsb /\
+        s = M.union sa sb /\ ls = composeLabels lsa lsb.
+  Proof.
+    induction 1.
+    - do 2 (eexists; exists nil); repeat split; try constructor.
+      subst.
+      admit. (* map stuff *)
+
+    - intros; subst.
+      specialize (IHMultistep eq_refl).
+      destruct IHMultistep as [sa [lsa [sb [lsb ?]]]]; dest; subst.
+
+      apply step_split in HStep.
+      destruct HStep as [soa [sob [sua [sub [sla [slb ?]]]]]]; dest; subst.
+
+      exists (M.union sua sa), (sla :: lsa).
+      exists (M.union sub sb), (slb :: lsb).
+      repeat split.
+
+      + constructor; auto.
+        admit. (* map stuff *)
+      + constructor; auto.
+        admit. (* map stuff *)
+      + admit. (* map stuff *)
+  Qed.
+
+  Lemma behavior_split:
+    forall s ls,
+      Behavior (ConcatMod ma mb) s ls ->
+      exists sa lsa sb lsb,
+        Behavior ma sa lsa /\ Behavior mb sb lsb /\
+        s = M.union sa sb /\
+        ls = composeLabels lsa lsb. 
+  Proof.
+    induction 1.
+    apply multistep_split in HMultistepBeh.
+    destruct HMultistepBeh as [sa [lsa [sb [lsb [? [? [? ?]]]]]]]; subst.
+    exists sa, lsa, sb, lsb.
+    repeat split; auto.
+    reflexivity.
+  Qed.
+
+  Lemma behavior_modular:
+    forall sa sb lsa lsb,
+      Behavior ma sa lsa ->
+      Behavior mb sb lsb ->
+      Behavior (ConcatMod ma mb) (M.union sa sb) (composeLabels lsa lsb).
+  Proof.
+    admit.
+  Qed.
+
+End TwoModules.
 
 Lemma equivalentLabel_hide_mergeLabel:
   forall p la lb,
